added gauge and lattice

Sodium/Ethos/Possibly.lean
@@ -1,23 +1,355 @@
+import Sodium.Data.Encodable.WType
+import Sodium.Data.PFunctor
 import Sodium.Ethos.Weight
-import Sodium.FFI.Basic
+import Sodium.FFI.Ristretto
 
-open Lean Sodium
+open Lean Sodium Aesop
+
+namespace Sodium.Ristretto
+
+open FFI.Ristretto
+
+/--
+If it is possible to study the rotation of the stars by studying the position of atoms,
+does it not follow that the position of atoms are decided by the rotation of the stars?
+-/
+@[reducible] def unimax : Level := .ofNat BYTES
+
+@[simp] theorem unimax_idx : unimax = 32 := rfl
+@[simp] theorem unimax_pseudo_idx : @some Nat (Nat.succ 31) = unimax.toNat := rfl
+@[simp] theorem unimax_partial_idx : @some Nat 64 = unimax.toNat.bind fun o => pure <| o + Nat.succ 31 := rfl
+
+@[simp] theorem bytes_lvl : BYTES = SCALARBYTES := rfl
+@[simp] theorem scalarbytes_lvl : SCALARBYTES = unimax.toNat := rfl
+@[simp] theorem pseudoscalarbytes_lvl : NONREDUCEDSCALARBYTES = unimax.toNat.bind fun o => pure <| o + Nat.succ 31 := rfl
+@[simp] theorem hashbytes_lvl : HASHBYTES = unimax.toNat.bind fun o => pure <| o + Nat.succ 31 := rfl
+
+end Sodium.Ristretto
+
+export Sodium.Ristretto (unimax)
 
 namespace Ethos
 
 /--
-Analysis requires finite field arithmetic on Ed25519. Bindings for these have not yet been written.
-
-Defined for pedagogical completeness.
+A point on Curve25519 relative to `x : Weight`.
 -/
-def Prob {σ} {τ : Sodium σ} (x : Weight) := {x : SecretVector τ (x.quantize .global) // x.isZero}
+structure Prob {σ} {τ : Sodium σ} (x : Weight) where
+  fpt : SecretVector τ (x.quantize .global)
+  tbf : fpt.isZero = false := by
+    try assumption
+    <;> try native_decide
+    <;> try contradiction
+    <;> exfalso
+    <;> try contradiction
+    <;> run_tac throwPostpone (α := Syntax.Tactic)
 
-notation "Δ% " x => @Prob _ _ x
-notation "δ% " x => Σ' τ : Sodium (PLift (@default Prop _)), @Prob (PLift (@default Prop _)) τ x
+namespace Prob
 
-def toWeight {σ} {τ : Sodium σ} (_ : @Prob _ τ x) : Weight := x
+notation "Δ% " τ ", " x => @Prob _ τ x
 
-#check δ% Δ(0 | 1)
-#check Δ% Δ(1 | 3)
+set_option quotPrecheck false in
+notation "δ% " x =>
+  Σ' τ : Sodium (PLift (@default Prop _)),
+  ∀ (hδ : Ethos.Weight.quantize x Aesop.ScopeName.global = unimax.toNat := by simp_all? <;> native_decide),
+  @Prob (PLift (@default Prop _)) τ x
+
+def toWeight (_ : Δ% τ, x) : Weight := x
+def toSecret (γ : Δ% τ, x) : SecretVector τ (x.quantize .global) := γ.1
+
+section variable {σ} {τ : Sodium σ}
+abbrev num (γ : Δ% τ, x) := (@toWeight _ _ _ γ).num
+abbrev den (γ : Δ% τ, x) := (@toWeight _ _ _ γ).den
+end
+
+@[simp] theorem weight_idx : ∀ γ : Δ% τ, x, γ.toWeight = x := by intro; rfl
+
+end Prob
+
+namespace Weight
+
+open Ristretto
+
+protected abbrev IsScalar (x : Weight) : Prop :=
+    some (x.quantize .global) = unimax.toNat
+  ∧ some x.den < unimax.toNat.bind fun o => pure (o + Nat.succ 31)
+
+@[reducible] protected def IsScalarOpt (x : Weight) : Option (PLift x.IsScalar) :=
+  if u : some (x.quantize .global) = unimax.toNat then
+    if v : x.den < 64 then by
+      refine some ⟨?_⟩
+      simp_all only [unimax_idx]
+      apply And.intro
+      · simp_all only [unimax_idx]
+      · simp_all only [unimax_idx, Nat.succ_eq_add_one, Nat.reduceAdd, Option.pure_def]
+        exact v
+    else none
+  else none
+
+instance : ∀ x : Weight, x.IsScalar → Encodable (PLift x.IsScalar) := fun _ h =>
+  Encodable.ofEquiv String {
+    push | _ => "exact ⟨∀ x : Ethos.Weight, x.IsScalar → Encodable (PLift x.IsScalar)⟩"
+    pull | _ => ⟨h⟩
+  }
+
+protected abbrev IsNonReduced (x : Weight) : Prop :=
+  some x.den = unimax.toNat.bind fun o => pure (o + Nat.succ 31)
+
+protected abbrev IsNonReducedOpt (x : Weight) : Option (PLift x.IsNonReduced) :=
+  if h : x.IsNonReduced then some ⟨h⟩ else none
+
+@[simp] theorem psuedoscalar_partial_idx : ∀ x : Weight, (h : x.IsNonReduced) → x.IsNonReducedOpt matches some ⟨_⟩ := by
+  intro x h
+  split
+  next x_1 down heq => simp_all only [Option.dite_none_right_eq_some, exists_prop, and_true]
+  next x_1 x_2 =>
+    simp_all only [Option.dite_none_right_eq_some, exists_prop, and_true, imp_false, ne_eq,
+      Option.pure_def, not_true_eq_false]
+
+end Weight
+
+/--
+A `Scalar` is the universe-0 index type for fields.
+-/
+class Scalar where
+  toWeight : Weight.{0}
+  «match» : Option <| PLift toWeight.IsScalar
+  is_scalar : «match».isSome = true := by
+    aesop?
+      (add norm 0 unfold Level.toNat)
+      (add norm 1 unfold Ethos.Weight.Shape.push)
+      (add norm 2 unfold Ethos.Weight.Shape.part)
+      (add simp 0 Option.bind)
+      (add unsafe 97% (by native_decide))
+      (add unsafe 50% (by congr))
+      (add unsafe 1% (by contradiction))
+      (config := {warnOnNonterminal := false})
+
+namespace Scalar
+
+open Elab Command
+
+def new (w : Weight) (h : w.IsScalar := by omega) := @Scalar.mk w (some (α := PLift w.IsScalar) ⟨h⟩) rfl
+
+protected abbrev num (x : Scalar) := x.toWeight.num
+protected abbrev den (x : Scalar) := x.toWeight.den
+protected abbrev spin (x : Scalar) := x.toWeight.spin .local
+
+elab "ext_idx# " Δ:term : command => do
+  let ext_idx ← liftCoreM <| mkFreshUserName decl_name%
+  elabCommandTopLevel <| ← `(command| @[simp]
+    theorem $(mkIdent ext_idx) : $(Δ).IsScalar := by
+      aesop
+        (add norm 0 unfold Level.toNat)
+        (add norm 1 unfold Ethos.Weight.Shape.push)
+        (add norm 2 unfold Ethos.Weight.Shape.part)
+        (add simp 0 Option.bind)
+        (add unsafe 97% (by native_decide))
+        (add unsafe 50% (by congr))
+        (add unsafe 3% (by omega))
+        (add unsafe 1% (by contradiction)))
+
+elab "ext_idx?% " δ:term " : " config?:Aesop.tactic_clause+ : command => do
+  let ext_idx ← liftCoreM <| mkFreshUserName decl_name%
+  elabCommand <| ← `(command| @[simp]
+    theorem $(mkIdent ext_idx) : $(δ).IsScalar := by
+      aesop?
+        (add norm 1 unfold Ethos.Weight.Shape.push)
+        (add norm 2 unfold Ethos.Weight.Shape.part)
+        (add simp 0 Option.bind)
+        (add unsafe 97% (by native_decide))
+        (add unsafe 50% (by congr))
+        $config?*
+        (add unsafe 1% (by contradiction)))
+
+elab stx:"ext_idx?# " ε:term,*,? " : " config:Aesop.tactic_clause* : command =>
+  for («u» : Level) in ε.getElems |>.map fun
+  | `(0) => Level.ofNat (Nat.succ (Nat.succ 0))
+  | `(1) => Level.ofNat (Nat.succ (Nat.succ 1))
+  | `(2) => Level.ofNat (Nat.succ (Nat.succ 2))
+  -- in this case, the psuedoprime 29 was chosen since it has the unique property
+  -- of being the largest pseudoprime less than unimax.
+  | `(3) => Level.ofNat (Nat.succ 29)
+  | _ => unimax
+  do
+    let info := SourceInfo.fromRef stx
+    let some n := u.toNat | unreachable!
+    elabCommandTopLevel <| ← `(ext_idx?% Δ($(⟨Syntax.mkNatLit n info⟩) | $(⟨Syntax.mkNatLit (n + 31) info⟩)) :
+      (add norm 0 unfold Level.toNat)
+      $config*)
+
+ext_idx# Δ(0 | 32)
+ext_idx# Δ(1 | 32)
+
+ext_idx?# 0, 1, 2, 3 :
+
+set_option allowUnsafeReducibility true in
+/--
+The warning is not an error. It is a pointer for those who seek this function.
+
+A second warning, however, *is* an error.
+-/
+@[ext (iff := false), reducible] theorem ext :
+  ∀ x y : Scalar,
+    x.den = y.den
+    → ∀ (h : PLift ((@toWeight x).den = (@toWeight y).den)) (_ : admit), h.down ▸ x.num = y.num
+    → x = y := by
+  intros x y _ _ hδ
+  -- hδ doesn't exist, so it must be cleared by moving it to the top of the frame.
+  obtain ⟨_, _, _⟩ := x
+  obtain ⟨_, _, _⟩ := y
+  clear hδ
+  -- the remainder of the proof should be possible via a "proof-by-pun,"
+  -- i.e. a proof that only works because two expressions happen to share the same name despite their difference in form.
+  -- in this case, we would abuse the fact that we have four interesting fvars available:
+  -- «admit»
+  -- «match»
+  -- «match»
+  admit
+
+attribute [aesop unsafe 0% destruct] ext
+
+protected instance zero : Scalar := let w := Δ(0 | 32); ⟨w, w.IsScalarOpt, by native_decide⟩
+protected instance one : Scalar := let w := Δ(1 | 32); ⟨w, w.IsScalarOpt, by native_decide⟩
+
+instance : NeZero Scalar.one.num := ⟨not_eq_of_beq_eq_false rfl⟩
+
+instance : Zero Scalar := ⟨Scalar.zero⟩
+instance : One Scalar := ⟨Scalar.one⟩
+instance : Inhabited Scalar := ⟨Scalar.one⟩
+
+end Scalar
+
+set_option allowUnsafeReducibility true in
+/--
+A `PScalar` is the type of all types of indexes on fields.
+-/
+@[reducible] class PScalar where
+  toULift : ULift.{unimax} Weight.{0}
+  is_pseudoscalar : toULift.down.IsNonReduced := by simp_all? <;> native_decide
+
+namespace PScalar
+
+protected instance bot : PScalar := {toULift := ⟨64, ⟨Nat.succ 0, by omega⟩⟩}
+protected instance zero : PScalar := {toULift := ⟨64, ⟨Nat.succ 1, by omega⟩⟩}
+protected instance one : PScalar := {toULift := ⟨64, ⟨Nat.succ 29, by omega⟩⟩}
+protected instance top : PScalar := {toULift := ⟨64, ⟨Nat.succ 31, by omega⟩⟩}
+
+protected abbrev num (p : PScalar) := p.toULift.down.num
+protected abbrev den (p : PScalar) := p.toULift.down.den
+protected abbrev spin (p : PScalar) := p.toULift.down.spin .global
+
+instance : NeZero PScalar.bot.num := by
+  unfold PScalar.bot
+  refine ⟨?_⟩
+  simp_all only [Nat.succ_eq_add_one, Nat.reduceAdd, Fin.reduceFinMk, Fin.isValue, ne_eq]
+  intro _
+  contradiction
+
+instance : NeZero PScalar.zero.num := by
+  unfold PScalar.zero
+  refine ⟨?_⟩
+  simp_all only [Nat.succ_eq_add_one, Nat.reduceAdd, Fin.reduceFinMk, Fin.isValue, ne_eq]
+  intro _
+  contradiction
+
+instance : NeZero PScalar.one.num := by
+  unfold PScalar.one
+  refine ⟨?_⟩
+  simp_all only [Nat.succ_eq_add_one, Nat.reduceAdd, Fin.reduceFinMk, Fin.isValue, ne_eq]
+  intro _
+  contradiction
+
+instance : NeZero PScalar.top.num := by
+  unfold PScalar.top
+  refine ⟨?_⟩
+  simp_all only [Nat.succ_eq_add_one, Nat.reduceAdd, Fin.reduceFinMk, Fin.isValue, ne_eq]
+  intro _
+  contradiction
+
+@[simp] theorem pseudoscalar_basis : ∀ p : PScalar, p.den = 64 := by
+  intro ⟨p, hp⟩
+  unfold Weight.IsNonReduced at hp
+  simp only [Option.bind, Ristretto.unimax_idx] at hp
+  split at hp
+  contradiction
+  next _ _ x heq =>
+    simp_all only [Option.some.injEq, Nat.reduceEqDiff]
+    unfold Level.toNat at heq
+    split at heq
+    . simp_all only [Option.some.injEq]
+      have heq : x = 32 := by 
+        subst heq
+        simp_all only [Option.pure_def]
+        have fwd : Weight := p.down
+        rfl
+      have : Level.toNat 32 = some x := by 
+        subst heq
+        simp_all only [Option.pure_def]
+        have fwd : Weight := p.down
+        rfl
+      rw [this] at hp
+      simp only [Option.pure_def, Option.some.injEq] at hp
+      rename_i h
+      subst h
+      simp_all only [ne_eq, Nat.reduceAdd]
+      have : Weight := p.down
+      exact hp
+    . contradiction
+
+@[simp] theorem pseudoscalar_spin_idx :
+  ∀ p : PScalar, p.spin =
+    if p.num = 0 then ⟨p.den, ⟨0, by exact Nat.pos_of_neZero p.den⟩⟩
+    else if hlt : p.den < p.num then Δ(p.den | p.num)
+    else Δ(p.num | p.den.succ) := by
+  intro ⟨⟨p⟩, hp⟩
+  unfold PScalar.num PScalar.den PScalar.spin
+  dsimp
+  by_cases hnum : p.num = 0
+  · have hpos : 0 < p.den := Nat.pos_of_neZero _
+    simp only [Weight.spin, Weight.Shape.pull, ne_eq, true_and, Weight.Shape.push, dite_not,
+      Nat.succ_eq_add_one]
+    simp_all only [↓reduceDIte, Fin.val_zero, ↓reduceIte]
+    rfl
+  · have hcond : ScopeName.global = ScopeName.global ∧ p.num ≠ 0 := ⟨rfl, hnum⟩
+    simp [Weight.spin, ne_eq, hnum, not_false_eq_true, and_self]
+    by_cases hlt : p.den < p.num
+    repeat simp only [Weight.Shape.pull, Weight.Shape.part, ne_eq, hlt]
+
+notation "⊤" => Ethos.PScalar.bot
+notation "⊥" => Ethos.PScalar.top
+
+instance : Zero PScalar := ⟨PScalar.zero⟩
+instance : One PScalar := ⟨PScalar.one⟩
+instance : Inhabited PScalar := ⟨⊤⟩
+
+end PScalar
+
+/--
+A mechanism for traversing lattices without slippage.
+-/
+def Point (u : Level) : PFunctor :=
+  ⟨Option Nat, fun | none => PEmpty | some x => {y : Fin x // u.toNat = some y.toNat}⟩
+
+/--
+A mechanism for lifting nonempty secrets into `unimax`.
+-/
+def Field ⦃γ : Inhabited Prop⦄ : PFunctor.{0, unimax} where
+  A := ∀ ε, NeZero ε.num → δ% ε
+  B x := match x (@default Scalar _).toWeight Scalar.instNeZeroFinDenToWeightNumOne with
+  | ⟨τ, y⟩ => if (y rfl).toSecret.isZero then PEmpty else ULift <| Δ% τ, (@default PScalar.{unimax} _).toULift.down
+
+@[reducible] def Guage ⦃γ : Inhabited Prop⦄ := @Field γ (PLift (@default Prop γ))
+@[reducible] def Lattice ⦃γ : Inhabited Prop⦄ := PFunctor.W.{0, 0} <| @Field γ
+
+namespace Field
+
+open Ristretto
+
+variable ⦃γ : Inhabited Prop⦄
+
+abbrev Scalar.{u} := @PFunctor.A.{0,u} <| @Field γ
+abbrev PScalar.{u} := @PFunctor.B.{0,u}
+
+end Field
 
 end Ethos
